{
 "cells": [
  {
   "cell_type": "markdown",
   "id": "160b7e8a-3b68-45c4-bf09-34ab131308c0",
   "metadata": {},
   "source": [
    "# 1.  Find the value of T(2) for the recurrence relation T(n) = 3T(n-1) + 12n, given that T(0)=5.\n",
    " \n",
    "Solution :-   \n",
    "\n",
    "To find the value of T(2) for the given recurrence relation \\( T(n) = 3T(n-1) + 12n \\), we can use the initial condition \\( T(0) = 5 \\).\n",
    "\n",
    "Given \\( T(n) = 3T(n-1) + 12n \\), let's first find \\( T(1) \\) using the recurrence relation:\n",
    "\n",
    "\\[ T(1) = 3T(1-1) + 12(1) = 3T(0) + 12 = 3(5) + 12 = 15 + 12 = 27 \\]\n",
    "\n",
    "Now, to find \\( T(2) \\):\n",
    "\n",
    "\\[ T(2) = 3T(2-1) + 12(2) = 3T(1) + 24 = 3(27) + 24 = 81 + 24 = 105 \\]\n",
    "\n",
    "So, the value of \\( T(2) \\) for the given recurrence relation is \\( \\boxed{105} \\).\n",
    "             "
   ]
  },
  {
   "cell_type": "markdown",
   "id": "4ba82538-8ef6-461d-907f-8647378758c8",
   "metadata": {},
   "source": [
    "## 2. Given a recurrence relation, solve it using the substitution method:\n",
    "\n",
    "# a. T(n) = T(n-1) + c\n",
    "\n",
    "if n = 1\n",
    "or n > 1\n",
    "\n",
    "Assume : T(1) = 1\n",
    "\n",
    "T(n-1) = T(n-1)-1 + c                   Put equation 1 in the given value\n",
    "T(n) = T(n-2) + c   (equation 1)   ,    T(n) = T(n-2) + 2c, we get.\n",
    "\n",
    "find next equation \n",
    "\n",
    "T(n-2) = T(n-3) + c  (equation 2)  ,    T(n) = T(n-3) + 3c, we get.\n",
    "\n",
    "now we repet it k times\n",
    "\n",
    "T(n) = T(n-k) + k.c               #(T(1) = 1)\n",
    "\n",
    "Find value of k, n-k = 1, k = n-1\n",
    "\n",
    "= T(1) + k.c\n",
    "= 1 + k.c \n",
    "put value of k,\n",
    "= 1 + (n-1).c\n",
    "= 1 + cn - c\n",
    "\n",
    "now c are the constant term then we get n\n",
    "\n",
    "Then the time complexity will be   O(n).\n",
    "\n"
   ]
  },
  {
   "cell_type": "markdown",
   "id": "185fbc3d-8303-4d2e-b2d5-2e7184e107e3",
   "metadata": {},
   "source": [
    "# b. T(n) = 2T(n/2) + n\n",
    "To solve the recurrence relation \\( T(n) = 2T(n/2) + n \\) using the substitution method, we'll follow these steps:\n",
    "\n",
    "1. Perform substitution repeatedly until we reach the base case.\n",
    "2. Use the base case to work backward and simplify the expression.\n",
    "\n",
    "Given the recurrence relation \\( T(n) = 2T(n/2) + n \\), let's start by substituting \\( n/2 \\) for \\( n \\) until we reach the base case:\n",
    "\n",
    "\\[\n",
    "\\begin{align*}\n",
    "T(n) &= 2T(n/2) + n \\\\\n",
    "&= 2[2T(n/4) + n/2] + n \\\\\n",
    "&= 2^2T(n/2^2) + 2n + n \\\\\n",
    "&= 2^2T(n/2^2) + 3n \\\\\n",
    "&= 2^2[2T(n/2^3) + n/2^2] + 3n \\\\\n",
    "&= 2^3T(n/2^3) + 3n + \\frac{3n}{2} \\\\\n",
    "&\\dots \\\\\n",
    "&= 2^kT(n/2^k) + kn\n",
    "\\end{align*}\n",
    "\\]\n",
    "\n",
    "We've reached \\( T(n/2^k) \\), which is typically the base case. Now, let's determine the value of \\( k \\) when \\( n/2^k = 1 \\):\n",
    "\n",
    "\\[\n",
    "\\frac{n}{2^k} = 1 \\implies n = 2^k \\implies k = \\log_2(n)\n",
    "\\]\n",
    "\n",
    "Using the base case \\( T(1) \\), we have:\n",
    "\n",
    "\\[\n",
    "T(1) = 2^kT(n/2^k) + kn = 2^{\\log_2(n)}T(1) + n \\log_2(n) = nT(1) + n \\log_2(n)\n",
    "\\]\n",
    "\n",
    "Given the base case \\( T(1) \\), typically \\( T(1) = \\text{constant} \\), we can say \\( T(1) = c \\). Therefore:\n",
    "\n",
    "\\[\n",
    "T(n) = nT(1) + n \\log_2(n) = cn + n \\log_2(n)\n",
    "\\]\n",
    "\n",
    "So, the solution to the recurrence relation \\( T(n) = 2T(n/2) + n \\) using the substitution method is cn + nlog_2(n)\n"
   ]
  },
  {
   "cell_type": "markdown",
   "id": "c4304eff-e3a5-47f8-8a1a-c22e27b25420",
   "metadata": {},
   "source": [
    "# c. T(n) = 2T(n/2) + c\n",
    "To solve the recurrence relation \\( T(n) = 2T(n/2) + c \\) using the substitution method, we'll follow similar steps as before:\n",
    "\n",
    "1. Perform substitution repeatedly until we reach the base case.\n",
    "2. Use the base case to work backward and simplify the expression.\n",
    "\n",
    "Given the recurrence relation \\( T(n) = 2T(n/2) + c \\), let's start by substituting \\( n/2 \\) for \\( n \\) until we reach the base case:\n",
    "\n",
    "\\[\n",
    "\\begin{align*}\n",
    "T(n) &= 2T(n/2) + c \\\\\n",
    "&= 2[2T(n/4) + c] + c \\\\\n",
    "&= 2^2T(n/2^2) + 2c + c \\\\\n",
    "&= 2^2T(n/2^2) + 3c \\\\\n",
    "&= 2^2[2T(n/2^3) + c] + 3c \\\\\n",
    "&= 2^3T(n/2^3) + 2^2c + 3c \\\\\n",
    "&\\dots \\\\\n",
    "&= 2^kT(n/2^k) + kc\n",
    "\\end{align*}\n",
    "\\]\n",
    "\n",
    "We've reached \\( T(n/2^k) \\), which is typically the base case. Now, let's determine the value of \\( k \\) when \\( n/2^k = 1 \\):\n",
    "\n",
    "\\[\n",
    "\\frac{n}{2^k} = 1 \\implies n = 2^k \\implies k = \\log_2(n)\n",
    "\\]\n",
    "\n",
    "Using the base case \\( T(1) \\), we have:\n",
    "\n",
    "\\[\n",
    "T(1) = 2^kT(n/2^k) + kc = 2^{\\log_2(n)}T(1) + c \\log_2(n) = nT(1) + c \\log_2(n)\n",
    "\\]\n",
    "\n",
    "Given the base case \\( T(1) \\), typically \\( T(1) = \\text{constant} \\), we can say \\( T(1) = c_1 \\). Therefore:\n",
    "\n",
    "\\[\n",
    "T(n) = nT(1) + c \\log_2(n) = c_1n + c \\log_2(n)\n",
    "\\]\n",
    "\n",
    "So, the solution to the recurrence relation \\( T(n) = 2T(n/2) + c \\) using the substitution method is c_1n + clog_2(n)"
   ]
  },
  {
   "cell_type": "markdown",
   "id": "fc47d67e-c713-42ce-9673-9a61941a561e",
   "metadata": {},
   "source": [
    "# d. T(n) = T(n/2) + c\n",
    "\n",
    "To solve the recurrence relation \\( T(n) = T(n/2) + c \\) using the substitution method, we'll proceed as follows:\n",
    "\n",
    "1. Perform substitution repeatedly until we reach the base case.\n",
    "2. Use the base case to work backward and simplify the expression.\n",
    "\n",
    "Given the recurrence relation \\( T(n) = T(n/2) + c \\), let's start by performing the substitution until we reach the base case:\n",
    "\n",
    "\\[ T(n) = T(n/2) + c \\]\n",
    "\n",
    "\\[ = [T(n/4) + c] + c \\]\n",
    "\n",
    "\\[ = T(n/4) + 2c \\]\n",
    "\n",
    "\\[ = [T(n/8) + c] + 2c \\]\n",
    "\n",
    "\\[ = T(n/8) + 3c \\]\n",
    "\n",
    "Continuing this process, after \\( k \\) steps, we get:\n",
    "\n",
    "\\[ T(n) = T(n/2^k) + kc \\]\n",
    "\n",
    "Now, let's find \\( k \\) such that \\( n/2^k = 1 \\):\n",
    "\n",
    "\\[ \\frac{n}{2^k} = 1 \\]\n",
    "\n",
    "\\[ n = 2^k \\]\n",
    "\n",
    "\\[ k = \\log_2(n) \\]\n",
    "\n",
    "Using the base case \\( T(1) \\), we have:\n",
    "\n",
    "\\[ T(1) = T(n/2^k) + kc = T(1) + c \\log_2(n) \\]\n",
    "\n",
    "\\[ T(1) = T(1) + c \\log_2(n) \\]\n",
    "\n",
    "\\[ 0 = c \\log_2(n) \\]\n",
    "\n",
    "\\[ \\log_2(n) = 0 \\]\n",
    "\n",
    "\\[ n = 2^0 \\]\n",
    "\n",
    "\\[ n = 1 \\]\n",
    "\n",
    "So, the base case is \\( T(1) \\). Given that \\( T(1) = c_0 \\) (a constant), we can conclude:\n",
    "\n",
    "\\[ T(n) = c_0 + c \\log_2(n) \\]\n",
    "\n",
    "So, the solution to the recurrence relation \\( T(n) = T(n/2) + c \\) using the substitution method is {c_0 + c \\log_2(n)"
   ]
  },
  {
   "cell_type": "markdown",
   "id": "6e3ab256-a58d-409e-b2fa-f65e5e37ef69",
   "metadata": {},
   "source": [
    "# 3. Given a recurrence relation, solve it using the recursive tree approach:"
   ]
  },
  {
   "cell_type": "markdown",
   "id": "a8557cea-9105-4261-b377-2e178728813c",
   "metadata": {},
   "source": [
    "# a. T(n) = 2T(n-1) +1\n",
    "\n",
    "To solve the recurrence relation \\(T(n) = 2T(n-1) + 1\\) using the recursive tree approach, we'll construct a tree to visualize the recursive calls and then sum up the costs at each level.\n",
    "\n",
    "1. **Constructing the Recursive Tree**:\n",
    "\n",
    "   At each level, the recurrence relation \\(T(n) = 2T(n-1) + 1\\) makes two recursive calls with \\(n-1\\) as the argument. Each node represents a recursive call, and the value associated with each node is the cost associated with that call.\n",
    "\n",
    "   Starting from \\(T(n)\\), we split into two branches: \\(T(n-1)\\) and \\(T(n-1)\\). Each of these branches further splits into two branches until we reach the base case.\n",
    "\n",
    "   Let's construct the first few levels of the tree:\n",
    "\n",
    "```\n",
    "                             T(n)\n",
    "                            /    \\\n",
    "                       T(n-1)   T(n-1)\n",
    "                      /    \\    /    \\\n",
    "                 T(n-2) T(n-2) T(n-2) T(n-2)\n",
    "                  / \\    / \\    / \\    / \\\n",
    "                ...  ... ... ... ... ... ...\n",
    "```\n",
    "\n",
    "2. **Analyzing the Tree**:\n",
    "\n",
    "   Each level of the tree corresponds to a different value of \\(n\\). At each level, there are \\(2^k\\) nodes, where \\(k\\) is the level of the tree. The cost associated with each node at level \\(k\\) is \\(2^k - 1\\) because every node except the root has a cost of 1.\n",
    "\n",
    "3. **Summing Up the Costs**:\n",
    "\n",
    "   To find the total cost, we sum up the costs at each level of the tree.\n",
    "\n",
    "   At level 1: \\(2^1 - 1 = 1\\)\n",
    "   At level 2: \\(2^2 - 1 = 3\\)\n",
    "   At level 3: \\(2^3 - 1 = 7\\)\n",
    "   At level \\(k\\): \\(2^k - 1\\)\n",
    "\n",
    "   We can see that at level \\(k\\), the cost is \\(2^k - 1\\).\n",
    "\n",
    "4. **Finding the Total Cost**:\n",
    "\n",
    "   The total cost is the sum of costs at each level up to level \\(n\\):\n",
    "\n",
    "   \\[ \\text{Total Cost} = \\sum_{k=1}^{n} (2^k - 1) \\]\n",
    "\n",
    "   This is a geometric series, and its sum is given by the formula:\n",
    "\n",
    "   \\[ \\text{Total Cost} = 2^{n+1} - n - 2 \\]\n",
    "\n",
    "So, using the recursive tree approach, the total cost of the recurrence relation \\(T(n) = 2T(n-1) + 1\\) is \\(2^{n+1} - n - 2\\)."
   ]
  },
  {
   "cell_type": "markdown",
   "id": "566daa07-5b00-4be3-a409-1b94d8cd1a2e",
   "metadata": {},
   "source": [
    "# b. T(n) = 2T(n/2) + n\n",
    "\n",
    "To solve the recurrence relation \\(T(n) = 2T(n/2) + n\\) using the recursive tree approach, we'll construct a tree to visualize the recursive calls and then sum up the costs at each level.\n",
    "\n",
    "1. **Constructing the Recursive Tree**:\n",
    "\n",
    "   At each level, the recurrence relation \\(T(n) = 2T(n/2) + n\\) makes two recursive calls with \\(n/2\\) as the argument. Each node represents a recursive call, and the value associated with each node is the cost associated with that call.\n",
    "\n",
    "   Starting from \\(T(n)\\), we split into two branches: \\(T(n/2)\\) and \\(T(n/2)\\). Each of these branches further splits into two branches until we reach the base case.\n",
    "\n",
    "   Let's construct the first few levels of the tree:\n",
    "\n",
    "```\n",
    "                             T(n)\n",
    "                            /    \\\n",
    "                       T(n/2)  T(n/2)\n",
    "                      /    \\    /    \\\n",
    "                  T(n/4) T(n/4) T(n/4) T(n/4)\n",
    "                  / \\    / \\    / \\    / \\\n",
    "                ...  ... ... ... ... ... ...\n",
    "```\n",
    "\n",
    "2. **Analyzing the Tree**:\n",
    "\n",
    "   Each level of the tree corresponds to a different value of \\(n\\). At each level, there are \\(2^k\\) nodes, where \\(k\\) is the level of the tree. The cost associated with each node at level \\(k\\) is \\(n/2^k\\) because every node at level \\(k\\) has \\(n/2^k\\) as the argument.\n",
    "\n",
    "3. **Summing Up the Costs**:\n",
    "\n",
    "   To find the total cost, we sum up the costs at each level of the tree.\n",
    "\n",
    "   At level 1: \\(n/2^1 = n/2\\)\n",
    "   At level 2: \\(n/2^2 = n/4\\)\n",
    "   At level 3: \\(n/2^3 = n/8\\)\n",
    "   At level \\(k\\): \\(n/2^k\\)\n",
    "\n",
    "4. **Finding the Total Cost**:\n",
    "\n",
    "   The total cost is the sum of costs at each level up to level \\(k = \\log_2 n\\), where \\(n\\) is the base case:\n",
    "\n",
    "   \\[ \\text{Total Cost} = n + \\frac{n}{2} + \\frac{n}{4} + \\ldots + 1 \\]\n",
    "\n",
    "   This is a geometric series with the first term \\(n\\) and the common ratio \\(1/2\\). The sum of such a series can be found using the formula for the sum of a geometric series:\n",
    "\n",
    "   \\[ \\text{Total Cost} = n \\left(1 + \\frac{1}{2} + \\frac{1}{4} + \\ldots + \\frac{1}{2^{\\log_2 n}} \\right) \\]\n",
    "\n",
    "   \\[ = n \\left(\\frac{1 - (1/2)^{\\log_2 n}}{1 - 1/2} \\right) \\]\n",
    "\n",
    "   \\[ = n \\left(\\frac{1 - 1/n}{1/2} \\right) \\]\n",
    "\n",
    "   \\[ = n \\times 2 \\left(1 - \\frac{1}{n}\\right) \\]\n",
    "\n",
    "   \\[ = 2n - 2 \\]\n",
    "\n",
    "So, using the recursive tree approach, the total cost of the recurrence relation \\(T(n) = 2T(n/2) + n\\) is \\(2n - 2\\)."
   ]
  },
  {
   "cell_type": "code",
   "execution_count": null,
   "id": "584f62e5-010b-4b38-96f4-e50b2fb8141a",
   "metadata": {},
   "outputs": [],
   "source": []
  }
 ],
 "metadata": {
  "kernelspec": {
   "display_name": "Python 3 (ipykernel)",
   "language": "python",
   "name": "python3"
  },
  "language_info": {
   "codemirror_mode": {
    "name": "ipython",
    "version": 3
   },
   "file_extension": ".py",
   "mimetype": "text/x-python",
   "name": "python",
   "nbconvert_exporter": "python",
   "pygments_lexer": "ipython3",
   "version": "3.10.8"
  }
 },
 "nbformat": 4,
 "nbformat_minor": 5
}
